Domain.lean
@@ -146,4 +146,5 @@ import Domain.Neighborhood.Theorem75
 import Domain.Neighborhood.Theorem76
 import Domain.Neighborhood.Proposition77
 import Domain.Neighborhood.Combinators77
+import Domain.Neighborhood.Example78
 import Domain.InfoSys
